IMP--_To_SAS+/Reduction.thy
@@ -11,19 +11,6 @@ type_synonym operator = "(variable, domain_element) sas_plus_operator"
 type_synonym state = "(variable, domain_element) state"
 type_synonym problem = "(variable, domain_element) sas_plus_problem"
 
-fun all_variables :: "com \<Rightarrow> vname list" where
-"all_variables (SKIP) = []" |
-"all_variables (Assign v aexp) = [ v ] @ (case aexp of 
-  A a \<Rightarrow> (case a of V v2 \<Rightarrow> [ v2 ] | N _ \<Rightarrow> []) |
-  Plus a b \<Rightarrow> [ a ] |
-  Sub a b \<Rightarrow> [ a ])" |
-"all_variables (c1 ;; c2) = all_variables c1 @ all_variables c2" |
-"all_variables (If v c1 c2) = [ v ] @ all_variables c1 @ all_variables c2" |
-"all_variables (While v c) = [ v ] @ all_variables c"
-
-definition enumerate_variables :: "com \<Rightarrow> vname list" where
-"enumerate_variables c = remdups (all_variables c)"
-
 fun all_subprograms :: "com \<Rightarrow> com list" where
 "all_subprograms (SKIP) = [SKIP]" |
 "all_subprograms (Assign v aexp) = [(Assign v aexp), SKIP]" |
@@ -35,6 +22,19 @@ fun all_subprograms :: "com \<Rightarrow> com list" where
 
 definition enumerate_subprograms :: "com \<Rightarrow> com list" where
 "enumerate_subprograms c = remdups (all_subprograms c)"
+
+fun all_variables :: "com \<Rightarrow> vname list" where
+"all_variables (SKIP) = []" |
+"all_variables (Assign v aexp) = [ v ] @ (case aexp of 
+  A a \<Rightarrow> (case a of V v2 \<Rightarrow> [ v2 ] | N _ \<Rightarrow> []) |
+  Plus a b \<Rightarrow> [ a ] |
+  Sub a b \<Rightarrow> [ a ])" |
+"all_variables (c1 ;; c2) = []" |
+"all_variables (If v c1 c2) = [ v ]" |
+"all_variables (While v c) = [ v ]"
+
+definition enumerate_variables :: "com \<Rightarrow> vname list" where
+"enumerate_variables c = remdups (concat (map all_variables (enumerate_subprograms c)))"
 
 declare enumerate_subprograms_def[simp] 
 
@@ -116,15 +116,66 @@ next
     by blast
 qed
 
+lemma SKIP_in_enumerate_subprograms[simp]: "SKIP \<in> set (enumerate_subprograms c)" 
+  by (induction c rule: all_subprograms.induct) auto
+
+lemma enumerate_subprogams_enumerate_variables: "c' \<in> set (enumerate_subprograms c) 
+  \<Longrightarrow> set (all_variables c') \<subseteq> set (enumerate_variables c)" 
+  by (auto simp: enumerate_variables_def)
+
+fun index_of :: "'a list \<Rightarrow> 'a \<Rightarrow> nat" where
+"index_of [] c = 0" |
+"index_of (d # cs) c = (if d = c then 0 else Suc (index_of cs c))"
+
+lemma index_of_element_in_list:
+  "x \<in> set l \<Longrightarrow> index_of l x < length l"
+  by (induction l) auto
+
+lemma index_of_identity[simp]:
+  "x \<in> set l \<Longrightarrow> (l ! (index_of l x) = x)"
+  by (induction l) auto
+
+fun index_of2 :: "('a \<times> 'b) list \<Rightarrow> 'a \<Rightarrow> nat" where
+"index_of2 [] c = 0" |
+"index_of2 ((d,_) # cs) c = (if d = c then 0 else Suc (index_of2 cs c))" 
+
+lemma index_of2_in_list: "x \<in> set (map fst l) \<Longrightarrow> (\<forall>y. (x, y) \<in> set l \<longrightarrow> P y) 
+  \<Longrightarrow> P (snd (l ! (index_of2 l x)))"
+  apply (induction l) 
+   apply auto
+  by force
+
+lemma index_of2_distinct: "(x, y) \<in> set l \<Longrightarrow> distinct (map fst l) 
+  \<Longrightarrow> l ! (index_of2 l x) = (x, y)"
+  apply(induction l)
+   apply(auto)
+  by force
+
 definition pc_to_com :: "com list \<Rightarrow> (variable \<times> domain_element) list \<Rightarrow> com" where
-"pc_to_com cs as = cs ! (case snd (the (find (\<lambda> i. fst i = PC) as)) of Num x \<Rightarrow> x | \<omega> \<Rightarrow> 0)" 
+"pc_to_com cs as = cs ! (case snd (as ! (index_of2 as PC)) of Num x \<Rightarrow> x)"
 
+lemma index_of2_index_of2[simp]: "x \<in> set (map fst l) 
+  \<Longrightarrow> l[index_of2 l x := (x, y)] ! index_of2 (l[index_of2 l x := (x, y)]) x = (x, y)"
+proof (induction l)
+  case (Cons a l)
+  then have "fst a = x \<or> fst a \<noteq> x" by simp
+  then show ?case
+  proof (elim disjE)
+    assume "fst a = x"
+    then show ?thesis using Cons 
+      by (metis eq_fst_iff index_of2.simps length_map length_pos_if_in_set list_update_code nth_list_update)
+  next
+    assume "fst a \<noteq> x"
+    then show ?thesis using Cons 
+      by (metis index_of2.simps list.simps(9) list_update_code nth_Cons_Suc prod.collapse set_ConsD)
+  qed
+qed auto
 
-definition index_of :: "'a list \<Rightarrow> 'a \<Rightarrow> nat" where
-"index_of cs c = snd (the (find (\<lambda> i. fst i = c) (zip cs [0..<(length cs)])))"
+lemma pc_to_com_of_subprogram: "c1 \<in> set cs \<Longrightarrow> PC \<in> set (map fst as) 
+  \<Longrightarrow> pc_to_com cs
+    (as [index_of2 as PC := (PC, Num (index_of cs c1))]) = c1"
+  by (induction cs) (auto simp: pc_to_com_def)
 
-definition index_of2 :: "('a \<times> 'b) list \<Rightarrow> 'a \<Rightarrow> nat" where
-"index_of2 cs c = snd (the (find (\<lambda> i. fst (fst i) = c) (zip cs [0..<(length cs)])))"
 
 fun com_to_operators :: "com list \<Rightarrow> com \<Rightarrow> domain_element list \<Rightarrow> operator list" where
 "com_to_operators cs (SKIP) d = []" |
@@ -132,24 +183,28 @@ fun com_to_operators :: "com list \<Rightarrow> com \<Rightarrow> domain_element
   (case aexp of
     A a \<Rightarrow> (case a of
       N val \<Rightarrow> [\<lparr> precondition_of = [(PC, Num i)], 
-                  effect_of = [(PC, Num j), (VN v, Num val)]\<rparr>] |
+                  effect_of = [(PC, Num j), (VN v, (if (Num val) \<in> set d then Num val else \<omega>))]\<rparr>] |
       V var \<Rightarrow> map (\<lambda> x. \<lparr> precondition_of = [(PC, Num i), (VN var, x)], 
                            effect_of = [(PC, Num j), (VN v, x)]\<rparr>) d) |
     Plus a b \<Rightarrow> map (\<lambda> x.  \<lparr> precondition_of = [(PC, Num i), (VN a, x)], 
-                             effect_of = [(PC, Num j), (VN v, (case x of Num y \<Rightarrow> Num (y + b) | \<omega> \<Rightarrow> \<omega>))]\<rparr>) d | 
+                             effect_of = [(PC, Num j), (VN v, (case x of 
+      Num y \<Rightarrow> if Num (y + b) \<in> set d then Num (y + b) else \<omega> | 
+      \<omega> \<Rightarrow> \<omega>))]\<rparr>) d | 
     Sub a b \<Rightarrow> map (\<lambda> x.  \<lparr> precondition_of = [(PC, Num i), (VN a, x)], 
-                            effect_of = [(PC, Num j), (VN v, (case x of Num y \<Rightarrow> Num (y - b) | \<omega> \<Rightarrow> \<omega>))]\<rparr>) d))" |
+                            effect_of = [(PC, Num j), (VN v, (case x of 
+      Num y \<Rightarrow> if Num (y - b) \<in> set d then Num (y - b) else \<omega> | 
+      \<omega> \<Rightarrow> \<omega>))]\<rparr>) d))" |
 "com_to_operators cs (c1;; c2) d = (let i = index_of cs (c1 ;; c2) in 
   (if c1 = SKIP then (let j = index_of cs c2 in [\<lparr> precondition_of = [(PC, Num i)],
-                                                  effect_of = [(PC, Num j)]\<rparr>])
+                                                   effect_of = [(PC, Num j)]\<rparr>])
    else (let ops = com_to_operators cs c1 d in map (\<lambda> op. 
-    (let j = index_of cs (pc_to_com cs (sas_plus_operator.effect_of op)) in 
+    (let j = index_of cs ((pc_to_com cs (effect_of op) ;; c2)) in 
       \<lparr> precondition_of = 
-        list_update (sas_plus_operator.precondition_of op) 
-                    (index_of2 (sas_plus_operator.precondition_of op) PC) (PC, Num i),
+        list_update (precondition_of op) 
+                    (index_of2 (precondition_of op) PC) (PC, Num i),
         effect_of = 
-        list_update (sas_plus_operator.effect_of op) 
-                    (index_of2 (sas_plus_operator.effect_of op) PC) (PC, Num j)\<rparr>)) ops)))" |
+        list_update (effect_of op) 
+                    (index_of2 (effect_of op) PC) (PC, Num j)\<rparr>)) ops)))" |
 "com_to_operators cs (IF v\<noteq>0 THEN c1 ELSE c2) d = (let i = index_of cs (IF v\<noteq>0 THEN c1 ELSE c2) ;
   j = index_of cs c1 ; k = index_of cs c2 in map (\<lambda> x. 
     \<lparr> precondition_of = [(PC, Num i), (VN v, x)], 
@@ -158,6 +213,244 @@ fun com_to_operators :: "com list \<Rightarrow> com \<Rightarrow> domain_element
   j = index_of cs (c ;; (WHILE v\<noteq>0 DO c)); k = index_of cs SKIP in map (\<lambda> x. 
     \<lparr> precondition_of = [(PC, Num i), (VN v, x)], 
       effect_of = [(PC, (if x = Num 0 then Num k else Num j))]\<rparr>) d)"
+
+lemma PC_in_update: 
+"(PC, y1) \<in> set l \<Longrightarrow> (\<exists>y2. (PC, y2) \<in> set (list_update l (index_of2 l PC) (PC, y3)))" 
+proof (induction l)
+  case (Cons a l)
+  then show ?case 
+    by (metis index_of2.simps list.set_intros list.set_intros list_update_code list_update_code prod.collapse set_ConsD)
+qed auto
+
+lemma PC_in_effect_precondition: "op \<in> set (com_to_operators cs c d) 
+  \<Longrightarrow> (\<exists>y1 y2. (PC, y1) \<in> set (precondition_of op) \<and> (PC, y2) \<in> set (effect_of op))"
+proof(induction cs c d arbitrary: op rule: com_to_operators.induct)
+  case (2 cs v aexp d)
+  then show ?case by (cases aexp) (auto simp: Let_def split: atomExp.splits)
+next
+  case (3 cs c1 c2 d)
+  have "c1 = SKIP \<or> c1 \<noteq> SKIP" by simp
+  then show ?case using 3 PC_in_update by fastforce
+qed auto
+
+lemma update_PC_registers_unchanged: 
+    "{x \<in> set l. fst x \<noteq> PC} =  {x \<in> set (list_update l (index_of2 l PC) (PC, y)). fst x \<noteq> PC}"
+proof (induction l)
+  case Nil
+  then show ?case by auto
+next
+  case (Cons a l)
+  have "fst a = PC \<or> fst a \<noteq> PC" by auto
+  then show ?case
+  proof (elim disjE)
+    assume "fst a = PC" 
+    then show ?thesis 
+      by (metis (no_types, lifting) Collect_cong fst_conv index_of2.simps list.set_intros 
+         list_update_code prod.collapse set_ConsD)
+  next
+    assume "fst a \<noteq> PC"
+    then have "index_of2 (a#l) PC \<noteq> 0" by (metis index_of2.simps old.nat.distinct prod.collapse)
+    then show ?thesis using Cons 
+      by (smt Collect_cong index_of2.elims insert_iff list.inject list.set list_update_code mem_Collect_eq)
+  qed
+qed
+
+lemma com_to_operators_seq_registers:
+  assumes "c1 \<noteq> SKIP" and  "op \<in> set (com_to_operators cs (c1 ;; c2) d)" 
+    and "(VN x, y) \<in> set (precondition_of op) \<or> (VN x, y) \<in> set (effect_of op)"
+  shows "\<exists>op'. op' \<in> set (com_to_operators cs c1 d) 
+          \<and> ((VN x, y) \<in> set (precondition_of op') \<or> (VN x, y) \<in> set (effect_of op'))"
+proof -
+  let ?i = "index_of cs (c1 ;; c2)"
+  obtain op' where "op' \<in> set (com_to_operators cs c1 d) 
+    \<and> op = (let j = index_of cs ((pc_to_com cs (effect_of op') ;; c2)) in 
+      \<lparr> precondition_of = 
+        list_update (precondition_of op') 
+                    (index_of2 (precondition_of op') PC) (PC, Num ?i),
+        effect_of = 
+        list_update (effect_of op') 
+                    (index_of2 (effect_of op') PC) (PC, Num j)\<rparr>)" using assms by auto
+  moreover then have "(VN x, y) \<in> set (precondition_of op') \<or> (VN x, y) \<in> set (effect_of op')" 
+    using assms update_PC_registers_unchanged by fastforce
+  ultimately show ?thesis by auto
+qed
+
+lemma com_to_operators_registers_in_d: 
+  "op \<in> set (com_to_operators cs c d) 
+  \<Longrightarrow> ((VN x, y) \<in> set (precondition_of op) \<or> (VN x, y) \<in> set (effect_of op)) \<Longrightarrow> \<omega> \<in> set d 
+  \<Longrightarrow> y \<in> set d"
+proof (induction cs c d arbitrary: op rule: com_to_operators.induct)
+  case (2 cs v aexp d)
+  then show ?case by (auto simp: Let_def split: aexp.splits atomExp.splits if_splits domain_element.splits)
+next
+  case (3 cs c1 c2 d)
+  have "c1 = SKIP \<or> c1 \<noteq> SKIP" by simp
+  then show ?case
+  proof (elim disjE)
+    assume "c1 \<noteq> SKIP"
+    then show ?thesis using 3 com_to_operators_seq_registers by metis
+  next
+    assume "c1 = SKIP" 
+    then show ?thesis using 3 by auto
+  qed
+qed (auto simp: Let_def split: aexp.splits atomExp.splits if_splits)
+
+lemma update_index_of2_preserve_set:
+  "set (map fst l) = set (map fst (list_update l (index_of2 l x) (x, y)))"
+proof (induction l)
+  case (Cons a l)
+  then show ?case
+    by (metis eq_fst_iff index_of2.simps list.set list.simps list_update_code list_update_code surjective_pairing)
+qed auto
+
+lemma update_index_of2_preserve_distinct: "distinct (map fst l)
+  \<Longrightarrow> distinct (map fst (list_update l (index_of2 l x) (x, y)))"
+proof (induction l)
+  case Nil
+  then show ?case by auto
+next
+  case (Cons a l)
+  let ?l' = "list_update l (index_of2 l x) (x, y)"
+  have "fst a = x \<or> fst a \<noteq> x" by auto
+  then show ?case
+  proof(elim disjE)
+    assume "fst a = x"
+    then show ?thesis using Cons 
+      by (metis (no_types, lifting) eq_fst_iff index_of2.simps list_update_code map_update)
+  next
+    assume "fst a \<noteq> x"
+    then show ?thesis using Cons update_index_of2_preserve_set 
+      by (metis card_distinct distinct_card length_list_update length_map)
+  qed
+qed
+
+lemma com_to_operators_variables_distinct: 
+  "op \<in> set (com_to_operators cs c d) \<Longrightarrow> (l = precondition_of op \<or> l = effect_of op)
+  \<Longrightarrow> distinct (map fst l)"
+proof(induction cs c d arbitrary: op l rule: com_to_operators.induct)
+  case (3 cs c1 c2 d)
+  have "c1 = SKIP \<or> c1 \<noteq> SKIP" by simp
+  then show ?case using 3 update_index_of2_preserve_distinct by fastforce
+qed (auto simp: Let_def split: aexp.splits atomExp.splits if_splits)
+
+lemma com_to_operators_PC_is_subprogram: 
+  "cs = enumerate_subprograms c \<Longrightarrow> c1 \<in> set cs \<Longrightarrow> op \<in> set (com_to_operators cs c1 d)
+  \<Longrightarrow> ((PC, y) \<in> set (precondition_of op) \<or> (PC, y) \<in> set (effect_of op))
+  \<Longrightarrow>  (pc_to_com cs (precondition_of op) \<in> set (enumerate_subprograms c1)
+      \<and> pc_to_com cs (effect_of op) \<in> set (enumerate_subprograms c1)
+      \<and> y \<in> set (map (\<lambda> i. Num i) [0..<(length cs)]))"
+proof (induction cs c1 d arbitrary: y op rule: com_to_operators.induct)
+  case (2 cs v aexp d)
+  moreover then have "v ::= aexp \<in> set cs" and "SKIP \<in> set cs" 
+    using SKIP_in_enumerate_subprograms by blast+
+  ultimately show ?case 
+    by (auto simp: Let_def pc_to_com_def index_of_element_in_list split: aexp.splits atomExp.splits)
+next
+  case (3 cs c1 c2 d)
+  then have c1c2_in_cs: "c1 ;; c2 \<in> set (enumerate_subprograms c) 
+    \<and> c1 \<in> set (enumerate_subprograms (c1 ;; c2)) \<and> c2 \<in> set (enumerate_subprograms (c1 ;; c2))" 
+    using c_in_all_subprograms_c by auto
+  then have "c1 \<in> set (enumerate_subprograms c) \<and> c2 \<in> set (enumerate_subprograms c)" 
+    using enumerate_subprograms_transitive by blast
+  then have c1_in_cs: "c1 \<in> set cs" and c2_in_cs: "c2 \<in> set cs" using 3 by auto
+  then have "c1 = SKIP \<or> c1 \<noteq> SKIP" by auto
+  then show ?case
+  proof (elim disjE)
+    assume "c1 = SKIP"
+    then show ?thesis
+      using 3 c2_in_cs c_in_all_subprograms_c c1c2_in_cs 
+      by (auto simp: Let_def pc_to_com_def index_of_element_in_list)
+  next
+    assume a: "c1 \<noteq> SKIP"
+    moreover then obtain op' where op'_def: "op' \<in> set (com_to_operators cs c1 d)
+      \<and> precondition_of op = list_update (precondition_of op') 
+                    (index_of2 (precondition_of op') PC) (PC, Num (index_of cs (c1 ;; c2)))
+      \<and> effect_of op = list_update (effect_of op') 
+                      (index_of2 (effect_of op') PC) (PC, Num (index_of cs (pc_to_com cs (effect_of op') ;; c2)))"
+      using 3 a by (auto simp: Let_def)
+    moreover then obtain c3 where c3_def: "c3 = pc_to_com cs (effect_of op')" by auto
+    ultimately have "c3 \<in> set (enumerate_subprograms c1)" using 3 c1_in_cs
+      by (meson PC_in_effect_precondition)
+    then have "c3 ;; c2 \<in> set (enumerate_subprograms (c1 ;; c2))" by auto
+    then have *: "c3 ;; c2 \<in> set cs" and **: "c1 ;; c2 \<in> set cs" using enumerate_subprograms_transitive 
+      using 3 "3.prems"(1) c1c2_in_cs by (meson PC_in_effect_precondition)+
+    have ***: "PC \<in> set (map fst (precondition_of op'))" and ****: "PC \<in> set (map fst (effect_of op'))"
+      using PC_in_effect_precondition 3 op'_def by (metis in_set_zipE zip_map_fst_snd)+
+    have "pc_to_com cs (precondition_of op) = c1 ;; c2" 
+      using op'_def pc_to_com_of_subprogram[OF ** ***] by auto 
+    moreover have "pc_to_com cs (effect_of op) = c3 ;; c2"
+      using op'_def pc_to_com_of_subprogram[OF * ****] using c3_def by auto
+    moreover have "y = Num (index_of cs (c1 ;; c2)) \<or> y = Num (index_of cs (c3 ;; c2))" 
+      using 3 op'_def c3_def com_to_operators_variables_distinct *** ****
+      by (metis Pair_inject index_of2_distinct index_of2_index_of2)
+    ultimately show ?thesis 
+      using c_in_all_subprograms_c \<open>c3;; c2 \<in> set (enumerate_subprograms (c1;; c2))\<close> 3 *
+      by (auto simp: index_of_element_in_list)
+  qed
+next
+  case (4 cs v c1 c2 d)
+  let ?i = "IF v \<noteq>0 THEN c1 ELSE c2"
+  have "?i \<in> set (enumerate_subprograms c) \<and> c1 \<in> set (enumerate_subprograms ?i) \<and> c2 \<in> set (enumerate_subprograms ?i)" 
+    using 4 c_in_all_subprograms_c by auto
+  moreover then have "c1 \<in> set (enumerate_subprograms c) \<and> c2 \<in> set (enumerate_subprograms c)"
+    using enumerate_subprograms_transitive by blast
+  ultimately have "?i \<in> set cs \<and> c1 \<in> set cs \<and> c2 \<in> set cs" using 4 by auto
+  then show ?case using 4 c_in_all_subprograms_c 
+    by (auto simp: Let_def pc_to_com_def index_of_element_in_list) 
+next
+  case (5 cs v c1 d)
+  let ?w = "WHILE v \<noteq>0 DO c1"
+  have "?w \<in> set (enumerate_subprograms c) \<and> c1 ;; ?w \<in> set (enumerate_subprograms ?w)" 
+    using 5 c_in_all_subprograms_c by auto
+  moreover then have "c1 ;; ?w \<in> set (enumerate_subprograms c)"
+    using enumerate_subprograms_transitive by blast
+  ultimately have "?w \<in> set cs \<and> c1 ;; ?w \<in> set cs \<and> SKIP \<in> set cs" 
+    using 5 SKIP_in_enumerate_subprograms by auto
+  then show ?case using 5 c_in_all_subprograms_c 
+    by (auto simp: Let_def pc_to_com_def index_of_element_in_list) 
+qed auto
+
+lemma com_to_operators_variables_in_enumerate_variables: "cs = (enumerate_subprograms c) ==> c1 \<in> set cs
+  \<Longrightarrow> op \<in> set (com_to_operators cs c1 d)
+  \<Longrightarrow> ((VN x, y) \<in> set (precondition_of op) \<or> (VN x, y) \<in> set (effect_of op))
+  \<Longrightarrow> x \<in> set (enumerate_variables c)"
+proof (induction cs c1 d arbitrary: op rule: com_to_operators.induct)
+  case (1 cs d)
+  then show ?case by auto
+next
+  case (2 cs v aexp d)
+  then have "set (all_variables (v ::= aexp)) \<subseteq> set (enumerate_variables c)" 
+    using enumerate_subprogams_enumerate_variables by blast 
+  then show ?case using 2 by (auto simp: Let_def split: aexp.splits atomExp.splits if_splits) 
+next
+  case (3 cs c1 c2 d)
+  have "c1 = SKIP \<or> c1 \<noteq> SKIP" by auto
+  then show ?case
+  proof (elim disjE)
+    assume "c1 = SKIP"
+    then show ?thesis using 3 by auto
+  next
+    assume "c1 \<noteq> SKIP"
+    then obtain op' where "op' \<in> set (com_to_operators cs c1 d) 
+          \<and> ((VN x, y) \<in> set (precondition_of op') \<or> (VN x, y) \<in> set (effect_of op'))"
+      using 3 com_to_operators_seq_registers by presburger
+    moreover have "c1 ;; c2 \<in> set (enumerate_subprograms c) \<and> c1 \<in> set (enumerate_subprograms (c1 ;; c2))" 
+      using 3 c_in_all_subprograms_c by simp
+    moreover then have "c1 \<in> set (enumerate_subprograms c)" 
+      using 3 enumerate_subprograms_transitive by blast
+    ultimately show ?thesis using 3 \<open>c1 \<noteq> SKIP\<close> by blast
+  qed
+next
+  case (4 cs v c1 c2 d)
+  then have "set (all_variables (IF v \<noteq>0 THEN c1 ELSE c2)) \<subseteq> set (enumerate_variables c)" 
+    using enumerate_subprogams_enumerate_variables by blast 
+  then show ?case using 4 by (auto simp: Let_def split: aexp.splits atomExp.splits if_splits)
+next
+  case (5 cs v c' d)
+  then have "set (all_variables (WHILE v \<noteq>0 DO c')) \<subseteq> set (enumerate_variables c)" 
+    using enumerate_subprogams_enumerate_variables by blast
+  then show ?case using 5 by (auto simp: Let_def split: aexp.splits atomExp.splits if_splits)
+qed
 
 definition coms_to_operators :: "com list \<Rightarrow> domain_element list \<Rightarrow> operator list" where
 "coms_to_operators cs d = concat (map (\<lambda> c. com_to_operators cs c d) cs)"
@@ -172,11 +465,119 @@ definition state_by_pc_and_vars ::
 definition imp_minus_minus_to_sas_plus :: "com \<Rightarrow> (vname \<rightharpoonup> nat) \<Rightarrow> nat \<Rightarrow> problem" where
 "imp_minus_minus_to_sas_plus c vs t = (let cs = enumerate_subprograms c ; 
   d = domain c t ; 
-  pc_d = map (\<lambda> i. Num i) [0..<(length cs + 1)] in
+  pc_d = map (\<lambda> i. Num i) [0..<(length cs)] in
     \<lparr> variables_of = PC # (map (\<lambda> v. VN v) (enumerate_variables c)),
       operators_of = coms_to_operators cs d, 
       initial_of = state_by_pc_and_vars cs c vs d,
       goal_of = state_by_pc_and_vars cs SKIP Map.empty d,
-      range_of = map_of ((PC, pc_d) # map (\<lambda> v. (VN v, d)) (enumerate_variables c))\<rparr>)"
+      range_of = (map_of (map (\<lambda> v. (VN v, d)) (enumerate_variables c)))(PC \<mapsto> pc_d)\<rparr>)"
+
+lemma range_defined: 
+  assumes "v \<in> set (variables_of (imp_minus_minus_to_sas_plus c vs t))" 
+  shows "(\<exists>y. range_of (imp_minus_minus_to_sas_plus c vs t) v = Some y)"
+proof(cases v)
+  case (VN x)
+  then have *: "(VN x, domain c t) \<in> set (map (\<lambda> v. (VN v, domain c t)) (enumerate_variables c))" 
+    using assms by (auto simp: Let_def imp_minus_minus_to_sas_plus_def)    
+  then show ?thesis using VN by (simp add: Let_def imp_minus_minus_to_sas_plus_def) 
+       (smt Pair_inject * ex_map_conv map_of_SomeD weak_map_of_SomeI)
+next
+  case PC
+  then show ?thesis by (auto simp: imp_minus_minus_to_sas_plus_def Let_def)
+qed
+
+lemma range_non_empty: 
+  assumes "v \<in> set (variables_of (imp_minus_minus_to_sas_plus c vs t))" 
+  shows "(\<exists>y. y \<in> range_of' (imp_minus_minus_to_sas_plus c vs t) v)"
+proof (cases v)
+  case (VN x)
+  then have *: "(VN x, domain c t) \<in> set (map (\<lambda> v. (VN v, domain c t)) (enumerate_variables c))" 
+    using assms by (auto simp: Let_def imp_minus_minus_to_sas_plus_def)
+  then have "range_of (imp_minus_minus_to_sas_plus c vs t) v = Some (domain c t)" 
+    using VN by (simp add: Let_def imp_minus_minus_to_sas_plus_def) 
+       (smt Pair_inject * ex_map_conv map_of_SomeD weak_map_of_SomeI)
+  then have "\<omega> \<in> range_of' (imp_minus_minus_to_sas_plus c vs t) v" 
+    by (auto simp: domain_def range_of'_def)
+  then show ?thesis by auto
+next
+  case PC
+  let ?pc_d = "(map (\<lambda> i. Num i) [0..<(length (enumerate_subprograms c))])"
+  have "range_of (imp_minus_minus_to_sas_plus c vs t) v 
+    = Some ?pc_d"
+    using assms PC by (auto simp: Let_def imp_minus_minus_to_sas_plus_def)
+  then have "range_of (imp_minus_minus_to_sas_plus c vs t) v = Some ?pc_d" using PC by simp
+  moreover have "Num 0 \<in> set ?pc_d" using SKIP_in_enumerate_subprograms 
+    by (metis (no_types, lifting) add.left_neutral in_set_conv_nth length_map length_pos_if_in_set map_nth nth_map nth_upt)
+  ultimately have "Num 0 \<in> range_of' (imp_minus_minus_to_sas_plus c vs t) v"
+    by (auto simp: domain_def range_of'_def)
+  then show ?thesis by auto
+qed
+
+lemma map_of_variables: "x \<in> set l \<Longrightarrow> (map_of (map (\<lambda>v. (VN v, d)) l) (VN x)) = Some d"
+  by (induction l) auto
+
+lemma distinct_list_all: 
+  assumes "distinct (map fst l)" 
+  shows "list_all (\<lambda>(v, a). list_all (\<lambda>(v', a'). v \<noteq> v' \<or> a = a') l) l"
+proof -
+  have "(v1, a1) \<in> set l \<Longrightarrow> list_all (\<lambda>(v', a'). v1 \<noteq> v' \<or> a1 = a') l" for v1 a1
+  proof -
+    assume "(v1, a1) \<in> set l"
+    then have "(v2, a2) \<in> set l \<Longrightarrow> v1 \<noteq> v2 \<or> a1 = a2" for v2 a2 
+      using assms by (meson eq_key_imp_eq_value)
+    then show ?thesis using Ball_set_list_all by blast
+  qed
+  then show ?thesis
+    by (metis (no_types, lifting) case_prodI2 list.pred_set)
+qed 
+  
+
+lemma operators_valid: 
+  assumes "cs = enumerate_subprograms c" and "c1 \<in> set cs" and "d = domain c t"
+         and  "op \<in> set (com_to_operators cs c1 d)"
+  shows "is_valid_operator_sas_plus (imp_minus_minus_to_sas_plus c vs t) op" 
+proof -                   
+  let ?\<Psi> = "imp_minus_minus_to_sas_plus c vs t"
+  let ?pre = "precondition_of op" and ?eff = "effect_of op" and ?vs = "variables_of ?\<Psi>" 
+      and ?D = "range_of ?\<Psi>" and ?pc_d = "(map (\<lambda> i. Num i) [0..<(length (enumerate_subprograms c))])"
+
+  have *: "((VN x, a) \<in> set ?pre \<or> (VN x, a) \<in> set ?eff) \<Longrightarrow> x \<in> set (enumerate_variables c)" for x a 
+    using com_to_operators_variables_in_enumerate_variables[OF assms(1) assms(2) assms(4)] by auto
+  then have "((VN x, a) \<in> set ?pre \<or> (VN x, a) \<in> set ?eff) \<Longrightarrow> ListMem (VN x) ?vs" for x a 
+    by (auto simp: imp_minus_minus_to_sas_plus_def Let_def ListMem_iff)
+  moreover have "ListMem PC ?vs" by (auto simp: imp_minus_minus_to_sas_plus_def Let_def ListMem_iff)
+  ultimately have "((v, a) \<in> set ?pre \<or> (v, a) \<in> set ?eff) \<Longrightarrow> ListMem v ?vs" for v a by (cases v) auto
+  then have pre_in_range: "list_all (\<lambda>(v, a). ListMem v ?vs) ?pre" 
+    and eff_in_range: "list_all (\<lambda>(v, a). ListMem v ?vs) ?eff"  
+    by (metis (mono_tags, lifting) case_prodI2 list.pred_set)+
+
+  have "x \<in> set (enumerate_variables c) \<Longrightarrow> ?D (VN x) = Some d" for x
+    using assms(3) map_of_variables by (simp add: imp_minus_minus_to_sas_plus_def Let_def) fast
+  then have "((VN x, a) \<in> set ?pre \<or> (VN x, a) \<in> set ?eff) \<Longrightarrow> ?D (VN x) = Some d" for x a 
+    using * by (auto simp: imp_minus_minus_to_sas_plus_def Let_def)
+  then have "((VN x, a) \<in> set ?pre \<or> (VN x, a) \<in> set ?eff) \<Longrightarrow> ?D (VN x) = Some d \<and> a \<in> set d" for x a
+    by (metis assms(3) assms(4) com_to_operators_registers_in_d domain_def in_set_conv_decomp)
+  moreover have "((PC, a) \<in> set ?pre \<or> (PC, a) \<in> set ?eff) \<Longrightarrow> ?D PC = Some ?pc_d \<and> a \<in> set ?pc_d" for a
+    using com_to_operators_PC_is_subprogram assms
+    by (metis (no_types, lifting) fun_upd_apply imp_minus_minus_to_sas_plus_def sas_plus_problem.select_convs)
+  ultimately have "((v, a) \<in> set ?pre \<or> (v, a) \<in> set ?eff) \<Longrightarrow> (?D v \<noteq> None \<and> a \<in> set (the (?D v)))" for v a
+    by (cases v) auto
+  then have "((v, a) \<in> set ?pre \<or> (v, a) \<in> set ?eff) \<Longrightarrow> (?D v \<noteq> None \<and> ListMem a (the (?D v)))" for v a
+    by (simp add: ListMem_iff)
+  then have "list_all (\<lambda>(v, a). (?D v \<noteq> None) \<and> ListMem a (the (?D v))) ?pre" 
+    and "list_all (\<lambda>(v, a). (?D v \<noteq> None) \<and> ListMem a (the (?D v))) ?eff" 
+    using Ball_set_list_all by blast+
+
+  then show ?thesis 
+    using com_to_operators_variables_distinct assms distinct_list_all pre_in_range eff_in_range 
+    apply (auto simp: is_valid_operator_sas_plus_def Let_def) 
+     apply blast+ 
+    done
+qed
+
+lemma imp_minus_minus_to_sas_plus_valid: 
+  "is_valid_problem_sas_plus (imp_minus_minus_to_sas_plus c vs t)"
+  apply(auto simp: is_valid_problem_sas_plus_def Let_def range_defined list_all_def)
+  sorry
 
 end
